Switch compilation implemented and verified in Rocq
This replaces the previous implementation by verified validation.

common/Switch.v
@@ -2,23 +2,23 @@
 (*                                                                     *)
 (*              The Compcert verified compiler                         *)
 (*                                                                     *)
-(*          Xavier Leroy, INRIA Paris-Rocquencourt                     *)
+(*          Xavier Leroy, Collège de France and INRIA                  *)
 (*                                                                     *)
 (*  Copyright Institut National de Recherche en Informatique et en     *)
 (*  Automatique.  All rights reserved.  This file is distributed       *)
-(*  under the terms of the GNU Lesser General Public License as        *)
-(*  published by the Free Software Foundation, either version 2.1 of   *)
-(*  the License, or  (at your option) any later version.               *)
-(*  This file is also distributed under the terms of the               *)
-(*  INRIA Non-Commercial License Agreement.                            *)
+(*  under the terms of the GNU General Public License as published by  *)
+(*  the Free Software Foundation, either version 2 of the License, or  *)
+(*  (at your option) any later version.  This file is also distributed *)
+(*  under the terms of the INRIA Non-Commercial License Agreement.     *)
 (*                                                                     *)
 (* *********************************************************************)
 
 (** Multi-way branches (``switch'' statements) and their compilation
     to comparison trees. *)
 
-From Coq Require Import EqNat.
-Require Import Coqlib Maps Integers Values.
+From Coq Require Import Recdef FMaps FMapFacts Zwf.
+From Coq Require FMapAVL.
+Require Import Coqlib Ordered Integers Values.
 
 (** A multi-way branch is composed of a list of (key, action) pairs,
   plus a default action.  *)
@@ -51,10 +51,234 @@ Inductive comptree : Type :=
   | CTiflt (key: Z) (clt: comptree) (cge: comptree)
   | CTjumptable (ofs: Z) (sz: Z) (acts: list nat) (cother: comptree).
 
+(** ** Compilation of multi-way branches *)
+
+(** *** Normalization of a multi-way branch *)
+
+(** Normalization performs the following steps, which do not change
+    the semantics of a switch (according to [switch_target], but
+    facilitate compilation:
+-     remove duplicate cases, keeping only the first case for each key;
+-     eliminate cases that are beyond the range of values of the scrutinee;
+-     sort cases by increasing key.
+*)
+
+Module ZMap := FMapAVL.Make OrderedZ.
+Module ZMapF := FMapFacts.Facts ZMap.
+
+Fixpoint map_of_table (modulus: Z) (tbl: table) : ZMap.t nat :=
+  match tbl with
+  | nil => ZMap.empty nat
+  | (k1, a1) :: tbl =>
+      let tbl' := map_of_table modulus tbl in
+      if zle 0 k1 && zlt k1 modulus then ZMap.add k1 a1 tbl' else tbl'
+  end.
+
+Definition normalize_table (modulus: Z) (tbl: table) : table :=
+  ZMap.elements (map_of_table modulus tbl).
+
+(** *** Compile a multi-way branch as a jump table *)
+
+Section JUMP_TABLE.
+
+Variable dfl: nat.
+Variable max: Z.
+
+Function jump_table (min: Z) (l: list (Z * nat))
+                    {wf (Zwf_up (max + 1)) min} : list nat :=
+  if zle min max then
+    match l with
+    | nil => dfl :: jump_table (min + 1) nil
+    | (k, d) :: l' =>
+        if zeq k min
+        then d :: jump_table (min + 1) l'
+        else dfl :: jump_table (min + 1) l
+    end
+  else nil.
+Proof.
+- intros; red; lia.
+- intros; red; lia.
+- intros; red; lia.
+- apply Zwf_up_well_founded.
+Defined.
+
+End JUMP_TABLE.
+
+Definition compile_jumptable (dfl: nat) (tbl: table) (min max: Z) :=
+  CTjumptable min (max - min + 1) (jump_table dfl max min tbl) (CTaction dfl).
+
+(** *** Compile a multi-way branch as a binary decision tree *)
+
+(** Split a list in two halves of approximately the same length.
+    (The second half can have one more element than the first half.)   *)
+
+Section LIST_SPLIT.
+
+Context {A: Type}.
+
+Fixpoint split_rec (before: list A) (after: list A) (cursor: list A) :=
+  match after, cursor with
+  | a1 :: al, c1 :: c2 :: cl => split_rec (a1 :: before) al cl
+  | _, _ => (List.rev' before, after)
+  end.
+
+Definition split_in_half (l: list A) : list A * list A :=
+  split_rec nil l l.
+
+Lemma split_rec_eq:
+  forall after before cursor,
+  fst (split_rec before after cursor) ++ snd (split_rec before after cursor)
+  = List.rev before ++ after.
+Proof.
+  induction after as [|a1 al]; simpl; intros.
+- rewrite List.rev_alt; auto. 
+- destruct cursor as [| c1 [ |c2 cl]]; simpl.
+  + rewrite List.rev_alt; auto. 
+  + rewrite List.rev_alt; auto.
+  + rewrite IHal. simpl. rewrite app_ass. auto.
+Qed.
+
+Lemma split_in_half_eq:
+  forall l, fst (split_in_half l) ++ snd (split_in_half l) = l.
+Proof.
+  unfold split_in_half; intros. rewrite split_rec_eq. auto.
+Qed.
+
+Lemma split_rec_length:
+  forall after before cursor,
+  (  length (fst (split_rec before after cursor)) * 2 <= length before * 2 + length cursor
+  /\ length (snd (split_rec before after cursor)) * 2 <= length after * 2 - length cursor + 1)%nat.
+Proof.
+  assert (length_rev': forall (l: list A), length (rev' l) = length l).
+  { intros. unfold rev'; rewrite <- rev_alt. apply rev_length. }
+  induction after as [ | a1 after]; intros before cursor; simpl.
+- rewrite length_rev'; lia.
+- destruct cursor as [ | c1 [ | c2 cursor' ]]; simpl.
+  + rewrite length_rev'; lia.  
+  + rewrite length_rev'; lia.  
+  + specialize (IHafter (a1 :: before) cursor'). simpl length in IHafter. lia.
+Qed.
+
+Lemma split_in_half_length:
+  forall l,
+  (  length (fst (split_in_half l)) * 2 <= length l
+  /\ length (snd (split_in_half l)) * 2 <= length l + 1)%nat.
+Proof.
+  intros. unfold split_in_half.
+  specialize (split_rec_length l nil l). simpl; lia.
+Qed.
+
+Lemma split_in_half_length':
+  forall a1 a2 al,
+  let l := a1 :: a2 :: al in
+  (  0 < length (fst (split_in_half l)) < length l
+  /\ 0 < length (snd (split_in_half l)) < length l)%nat.
+Proof.
+  intros.
+  set (l1 := fst (split_in_half l)).
+  set (l2 := snd (split_in_half l)).
+  assert (L: (length l1 + length l2 = length l)%nat).
+  { rewrite <- app_length. unfold l1, l2; rewrite split_in_half_eq; auto. }
+  specialize (split_in_half_length l). fold l1; fold l2.
+  unfold l in *. simpl length in *. lia.
+Qed.
+
+End LIST_SPLIT.
+
+(** Compile a multi-way branch to a binary decision tree, using a variant
+    of binary search.  The base cases are branches with one, two, or three
+    branches, which are compiled to the minimal number of equality tests. *)
+
+Definition compile_tree_1 (dfl: nat) (k1: Z) (a1: nat) (min max: Z) : comptree :=
+  if zeq max min then
+    CTaction a1
+  else
+    CTifeq k1 a1 (CTaction dfl).
+
+Definition compile_tree_2 (dfl: nat) (k1: Z) (a1: nat) (k2: Z) (a2: nat) (min max: Z) : comptree :=
+  CTifeq k1 a1
+    (if zeq (max - min) 1 then
+      CTaction a2
+     else
+      CTifeq k2 a2 (CTaction dfl)).
+
+Definition compile_tree_3 (dfl: nat) (k1: Z) (a1: nat) (k2: Z) (a2: nat) (k3: Z) (a3: nat) (min max: Z) : comptree :=
+  CTifeq k1 a1
+    (CTifeq k2 a2
+      (if zeq (max - min) 2 then
+         CTaction a3
+       else
+         CTifeq k3 a3 (CTaction dfl))).
+
+Definition first_key (tbl: table) : Z :=
+  match tbl with
+  | nil => 0   (**r should not happen *)
+  | (key, act) :: tbl => key
+  end.
+
+Function compile_tree (dfl: nat) (tbl: table) (min max: Z)
+                      { measure length tbl } : comptree :=
+  match tbl with
+  | nil => CTaction dfl
+  | (k1, a1) :: nil =>
+       compile_tree_1 dfl k1 a1 min max
+  | (k1, a1) :: (k2, a2) :: nil =>
+       compile_tree_2 dfl k1 a1 k2 a2 min max
+  | (k1, a1) :: (k2, a2) :: (k3, a3) :: nil =>
+       compile_tree_3 dfl k1 a1 k2 a2 k3 a3 min max
+  | _ =>
+     let (tbl1, tbl2) := split_in_half tbl in
+     let pivot := first_key tbl2 in
+     CTiflt pivot (compile_tree dfl tbl1 min (pivot - 1))
+                  (compile_tree dfl tbl2 pivot max)
+  end.
+Proof.
+- intros.
+  destruct (split_in_half_length' (k1, a1) (k2, a2) ((k3, a3) :: p2 :: l2)) as [P Q].
+  rewrite teq6 in Q; tauto.
+- intros.
+  destruct (split_in_half_length' (k1, a1) (k2, a2) ((k3, a3) :: p2 :: l2)) as [P Q].
+  rewrite teq6 in P; tauto.
+Defined.
+
+(** *** Normalization and compilation to a decision tree *)
+
+(** Heuristic to choose between the two compilation strategies.
+    We estimate the code size (including the size of the jump table)
+    for the two strategies and choose the one with the smaller size.
+    Also, small jump tables are not efficient, so we always use
+    decision trees for 6 cases or less. *)
+
+Definition dense_enough (numcases span: Z) : bool :=
+  let tree_size := numcases * 4 in
+  let table_size := span + 8 in
+  zle 7 numcases
+  && zle table_size tree_size
+  && zlt span Int.modulus.
+
+(** The entry point: normalize and compile to a decision tree. *)
+
+Definition compile_switch (modulus: Z) (dfl: nat) (tbl: table) :=
+  let tbl1 := normalize_table modulus tbl in
+  match tbl1 with
+  | nil =>  CTaction dfl
+  | (kmin, _) as cmin :: _ =>
+      let (kmax, _) := List.last tbl1 cmin in
+      let numcases := list_length_z tbl1 in
+      if dense_enough numcases (kmax - kmin + 1)
+      then compile_jumptable dfl tbl1 kmin kmax
+      else compile_tree dfl tbl1 0 (modulus - 1)
+  end.
+
+(** ** Correctness proof *)
+
 Section COMPTREE.
 
 Variable modulus: Z.
 Hypothesis modulus_pos: modulus > 0.
+
+(** Semantics of decision trees.  The "modulo" computations in the [CTjumptable]
+  case reflect the use of machine integer arithmetic in the compiled code. *)
 
 Fixpoint comptree_match (n: Z) (t: comptree) {struct t}: option nat :=
   match t with
@@ -70,105 +294,8 @@ Fixpoint comptree_match (n: Z) (t: comptree) {struct t}: option nat :=
       else comptree_match n t'
   end.
 
-(** The translation from a table to a comparison tree is performed
-  by untrusted Caml code (function [compile_switch] in
-  file [Switchaux.ml]).  In Coq, we validate a posteriori the
-  result of this function.  In other terms, we now develop
-  and prove correct Coq functions that take a table and a comparison
-  tree, and check that their semantics are equivalent. *)
-
-Fixpoint split_lt (pivot: Z) (cases: table)
-                  {struct cases} : table * table :=
-  match cases with
-  | nil => (nil, nil)
-  | (key, act) :: rem =>
-      let (l, r) := split_lt pivot rem in
-      if zlt key pivot
-      then ((key, act) :: l, r)
-      else (l, (key, act) :: r)
-  end.
-
-Fixpoint split_eq (pivot: Z) (cases: table)
-                  {struct cases} : option nat * table :=
-  match cases with
-  | nil => (None, nil)
-  | (key, act) :: rem =>
-      let (same, others) := split_eq pivot rem in
-      if zeq key pivot
-      then (Some act, others)
-      else (same, (key, act) :: others)
-  end.
-
-Fixpoint split_between (dfl: nat) (ofs sz: Z) (cases: table)
-                       {struct cases} : ZMap.t nat * table :=
-  match cases with
-  | nil => (ZMap.init dfl, nil)
-  | (key, act) :: rem =>
-      let (inside, outside) := split_between dfl ofs sz rem in
-      if zlt ((key - ofs) mod modulus) sz
-      then (ZMap.set key act inside, outside)
-      else (inside, (key, act) :: outside)
-  end.
-
-Definition refine_low_bound (v lo: Z) :=
-  if zeq v lo then lo + 1 else lo.
-
-Definition refine_high_bound (v hi: Z) :=
-  if zeq v hi then hi - 1 else hi.
-
-Fixpoint validate_jumptable (cases: ZMap.t nat)
-                            (tbl: list nat) (n: Z) {struct tbl} : bool :=
-  match tbl with
-  | nil => true
-  | act :: rem =>
-      Nat.eqb act (ZMap.get n cases)
-      && validate_jumptable cases rem (Z.succ n)
-  end.
-
-Fixpoint validate (default: nat) (cases: table) (t: comptree)
-                  (lo hi: Z) {struct t} : bool :=
-  match t with
-  | CTaction act =>
-      match cases with
-      | nil =>
-          Nat.eqb act default
-      | (key1, act1) :: _ =>
-          zeq key1 lo && zeq lo hi && Nat.eqb act act1
-      end
-  | CTifeq pivot act t' =>
-      zle 0 pivot && zlt pivot modulus &&
-      match split_eq pivot cases with
-      | (None, _) =>
-          false
-      | (Some act', others) =>
-          Nat.eqb act act'
-          && validate default others t'
-                      (refine_low_bound pivot lo)
-                      (refine_high_bound pivot hi)
-      end
-  | CTiflt pivot t1 t2 =>
-      zle 0 pivot && zlt pivot modulus &&
-      match split_lt pivot cases with
-      | (lcases, rcases) =>
-          validate default lcases t1 lo (pivot - 1)
-          && validate default rcases t2 pivot hi
-      end
-  | CTjumptable ofs sz tbl t' =>
-      let tbl_len := list_length_z tbl in
-      zle 0 ofs && zlt ofs modulus &&
-      zle 0 sz && zlt sz modulus &&
-      zle (ofs + sz) modulus && zle sz tbl_len && zlt sz Int.modulus &&
-      match split_between default ofs sz cases with
-      | (inside, outside) =>
-          validate_jumptable inside tbl ofs
-          && validate default outside t' lo hi
-     end
-  end.
-
-Definition validate_switch (default: nat) (cases: table) (t: comptree) :=
-  validate default cases t 0 (modulus - 1).
-
-(** Structural properties checked by validation *)
+(** Well-formedness conditions on decision trees.  The integer literals mentioned
+  must be representable as machine integers. *)
 
 Inductive wf_comptree: comptree -> Prop :=
   | wf_action: forall act,
@@ -182,169 +309,454 @@ Inductive wf_comptree: comptree -> Prop :=
       wf_comptree cother ->
       wf_comptree (CTjumptable ofs sz acts cother).
 
-Lemma validate_wf:
-  forall default t cases lo hi,
-  validate default cases t lo hi = true ->
-  wf_comptree t.
+(** Tables that are sorted by strictly increasing keys. *)
+
+Inductive sorted: table -> Prop :=
+  | sorted_nil: sorted nil
+  | sorted_cons: forall k a tbl,
+      sorted tbl ->
+      (forall k' a', In (k', a') tbl -> k < k') ->
+      sorted ((k, a) :: tbl).
+
+Lemma sorted_app_inv:
+  forall tbl1 tbl2,
+  sorted (tbl1 ++ tbl2) ->
+  sorted tbl1 /\ sorted tbl2 /\
+  forall k1 a1 k2 a2, In (k1, a1) tbl1 -> In (k2, a2) tbl2 -> k1 < k2.
 Proof.
-  induction t; simpl; intros; InvBooleans.
+  induction tbl1 as [ | [k a] tbl1]; simpl; intros.
+- intuition auto. constructor.
+- inv H. exploit IHtbl1; eauto. intros (P & Q & R).
+  intuition eauto.
+  constructor. auto. eauto using in_or_app. inv H1; eauto using in_or_app. 
+Qed.
+
+Lemma in_sorted_le:
+  forall k a l k' a',
+  sorted ((k, a) :: l) -> In (k', a') ((k, a) :: l) -> k <= k'.
+Proof.
+  intros. inv H. simpl in H0; destruct H0.
+- inv H; lia.
+- assert (k < k') by eauto. lia.
+Qed.
+
+Lemma in_sorted_ge:
+  forall k a l k' a',
+  sorted (l ++ (k, a) :: nil) -> In (k', a') (l ++ (k, a) :: nil) -> k' <= k.
+Proof.
+  intros. exploit sorted_app_inv; eauto. intros (P & Q & R).
+  rewrite in_app_iff in H0. destruct H0.
+  assert (k' < k) by eauto with coqlib. lia.
+  simpl in H0; intuition auto. inv H1; lia.
+Qed.
+
+(** Properties of [switch_target] *)
+
+Lemma switch_target_app_2:
+  forall n dfl tbl2 tbl1,
+  (forall k a, In (k, a) tbl1 -> n <> k) ->
+  switch_target n dfl (tbl1 ++ tbl2) = switch_target n dfl tbl2.
+Proof.
+  induction tbl1; simpl; intros.
+- auto.
+- destruct a as [k1 a1]. rewrite zeq_false; eauto.
+Qed.
+
+Lemma switch_target_outside:
+  forall n dfl cases,
+  (forall k d, In (k, d) cases -> n <> k) ->
+  switch_target n dfl cases = dfl.
+Proof.
+  intros. rewrite <- (List.app_nil_r cases). apply switch_target_app_2; auto. 
+Qed.
+
+Lemma switch_target_app_1:
+  forall n dfl tbl2,
+  (forall k a, In (k, a) tbl2 -> n <> k) ->
+  forall tbl1,
+  switch_target n dfl (tbl1 ++ tbl2) = switch_target n dfl tbl1.
+Proof.
+  induction tbl1; simpl.
+- apply switch_target_outside; auto.
+- destruct a as (k1, a1). destruct (zeq n k1); auto.
+Qed.
+
+Lemma switch_target_sorted:
+  forall k a dfl tbl, sorted tbl -> In (k, a) tbl -> switch_target k dfl tbl = a.
+Proof.
+  induction 1; simpl; intros.
+- contradiction.
+- destruct H1.
+  + inv H1. apply zeq_true.
+  + rewrite zeq_false. eauto. apply H0 in H1; lia. 
+Qed.
+
+(** Correctness of normalization *)
+
+Lemma map_of_table_charact:
+  forall n dfl tbl,
+  0 <= n < modulus ->
+  match ZMap.find n (map_of_table modulus tbl) with
+  | Some a => a
+  | None => dfl
+  end = switch_target n dfl tbl.
+Proof.
+  induction tbl as [ | [k1 a1] tbl ]; simpl; intros.
+- auto.
+- destruct (zle 0 k1 && zlt k1 modulus) eqn:R; destruct (zeq n k1).
+  + subst n. rewrite ZMapF.add_eq_o; auto.
+  + rewrite ZMapF.add_neq_o; auto. 
+  + subst k1. unfold proj_sumbool in R; rewrite zle_true in R by tauto; rewrite zlt_true in R by tauto. discriminate.
+  + auto.
+Qed.
+
+Lemma map_of_table_wf:
+  forall k a tbl, ZMap.MapsTo k a (map_of_table modulus tbl) -> 0 <= k < modulus.
+Proof.
+  induction tbl as [ | [k1 a1] tbl]; simpl; intros.
+- eelim ZMap.empty_1; eauto.
+- destruct (zle 0 k1 && zlt k1 modulus) eqn:R; eauto.
+  rewrite ZMapF.add_mapsto_iff in H. destruct H as [[P Q] | [P Q]].
+  + subst k. InvBooleans. auto.
+  + eauto.
+Qed.
+
+Lemma normalize_table_wf:
+  forall tbl k a, In (k, a) (normalize_table modulus tbl) -> 0 <= k < modulus.
+Proof.
+  unfold normalize_table; intros.
+  apply map_of_table_wf with a tbl. 
+  apply ZMap.elements_2. rewrite InA_alt. exists (k, a); split; auto. 
+  hnf; auto.
+Qed.
+
+Lemma zmap_elements_sorted:
+  forall m, sorted (ZMap.elements m).
+Proof.
+  assert (forall l, Sorted (ZMap.lt_key (elt := nat)) l -> sorted l).
+  {
+    induction 1.
+  - constructor.
+  - destruct a as [k a]. inv H0.
+    + constructor. constructor. simpl; tauto.
+    + destruct b as [k' a']. assert (k < k') by auto. 
+      constructor; auto. intros k'' a'' IN. 
+      assert (k' <= k'') by (eapply in_sorted_le; eauto). 
+      lia.
+  }
+  intros. apply H. apply ZMap.elements_3. 
+Qed.
+
+Lemma normalize_table_sorted:
+  forall tbl, sorted (normalize_table modulus tbl).
+Proof.
+  intros; apply zmap_elements_sorted.
+Qed.
+
+Lemma switch_target_elements:
+  forall n dfl m,
+  switch_target n dfl (ZMap.elements m) = 
+  match ZMap.find n m with None => dfl | Some a => a end.
+Proof.
+  intros. destruct (ZMap.find n m) as [a|] eqn:F.
+- apply switch_target_sorted. apply zmap_elements_sorted. 
+  exploit ZMap.elements_1. apply ZMap.find_2; eauto. 
+  rewrite InA_alt. intros [[k2 a2] [[P Q] R]]. simpl in *; subst; auto.
+- apply switch_target_outside. intros. 
+  assert (ZMap.find k m = Some d). 
+  { apply ZMap.find_1. apply ZMap.elements_2. apply InA_alt.
+    exists (k,d); split; auto. reflexivity. }
+  congruence.
+Qed.
+
+Lemma normalize_table_correct:
+  forall n dfl tbl,
+  0 <= n < modulus ->
+  switch_target n dfl (normalize_table modulus tbl) = switch_target n dfl tbl.
+Proof.
+  intros. unfold normalize_table. rewrite switch_target_elements. 
+  apply map_of_table_charact; auto.
+Qed.
+
+(** Correctness of compilation to a jump table. *)
+
+Lemma nth_jump_table:
+  forall max n min dfl l,
+  sorted l ->
+  (forall k d, In (k, d) l -> min <= k <= max) ->
+  min <= n <= max ->
+  list_nth_z (jump_table dfl max min l) (n - min) = Some (switch_target n dfl l).
+Proof.
+  intros until l.
+  functional induction (jump_table dfl max min l); intros SS R1 R2.
+- simpl list_nth_z. destruct (zeq (n - min) 0); auto.
+  replace (Z.pred (n - min)) with (n - (min + 1)) by lia.
+  apply IHl0. auto. simpl; tauto. lia.
+- simpl. inv SS. destruct (zeq (n - min) 0).
++ replace n with min by lia. rewrite zeq_true. auto.
++ rewrite zeq_false by lia.
+  replace (Z.pred (n - min)) with (n - (min + 1)) by lia.
+  apply IHl0. auto. 
+  intros. 
+  assert (min <= k <= max) by eauto with coqlib.
+  assert (min < k) by eauto.
+  lia.
+  lia.
+- simpl list_nth_z. destruct (zeq (n - min) 0).
++ inv SS. rewrite switch_target_outside; auto.
+  intros. 
+  replace n with min by lia.
+  assert (min <= k <= max) by eauto with coqlib. 
+  simpl in H. destruct H. inv H. lia. 
+  exploit H3; eauto. lia.
++ replace (Z.pred (n - min)) with (n - (min + 1)) by lia.
+  apply IHl0. auto. 
+  intros. exploit R1; eauto. intros.
+  simpl in H; destruct H.
+  inv H. lia.
+  inv SS. apply H5 in H. 
+  assert (min <= k <= max) by eauto with coqlib.
+  lia.
+  lia.
+- lia.
+Qed.
+
+Lemma compile_jumptable_correct:
+  forall n dfl tbl min max,
+  sorted tbl ->
+  (forall k a, In (k, a) tbl -> min <= k <= max) ->
+  0 <= min -> min <= max -> max < modulus -> 
+  max - min + 1 < Int.modulus ->
+  0 <= n < modulus ->
+  comptree_match n (compile_jumptable dfl tbl min max) = Some(switch_target n dfl tbl).
+Proof.
+  intros until max; intros SRT R1 R2 R3 R4 R5 R6.
+  unfold compile_jumptable. simpl. 
+  set (delta := n - min).
+  assert (-modulus < delta < modulus) by (unfold delta; lia).
+  destruct (zle 0 delta).
+- assert (E: delta mod modulus = delta).
+  { apply Zmod_small. lia. }
+  rewrite E. 
+  destruct (zlt delta (max - min + 1)).
++ assert (F: delta mod Int.modulus = delta).
+  { apply Zmod_small. lia. }
+  rewrite F. 
+  apply nth_jump_table; auto. unfold delta in *; lia. 
++ rewrite switch_target_outside; auto. 
+  intros. assert (min <= k <= max) by eauto. unfold delta in *; lia.
+- assert (E: delta mod modulus = delta + modulus).
+  { apply Zmod_unique with (-1). ring. lia. }
+  rewrite E.
+  assert (F: delta + modulus >= max - min + 1).
+  { unfold delta in *; lia. }
+  rewrite zlt_false by auto. rewrite switch_target_outside; auto.
+  intros. assert (min <= k <= max) by eauto. unfold delta in *; lia.
+Qed.
+
+Lemma compile_jumptable_wf:
+  forall dfl tbl min max,
+  0 <= min -> min <= max -> max < modulus -> 
+  max - min + 1 < Int.modulus -> Int.modulus <= modulus ->
+  wf_comptree (compile_jumptable dfl tbl min max).
+Proof.
+  intros; unfold compile_jumptable. constructor. lia. lia. constructor.
+Qed.
+
+(** Correctness of compilation to a decision tree *)
+
+Lemma compile_tree_1_correct:
+  forall dfl k1 a1 min max n,
+  (forall k a, In (k, a) ((k1, a1) :: nil) -> min <= k <= max) ->
+  min <= n <= max ->
+  comptree_match n (compile_tree_1 dfl k1 a1 min max) =
+  Some (switch_target n dfl ((k1, a1) :: nil)).
+Proof.
+  unfold compile_tree_1; intros.
+  assert (min <= k1 <= max) by eauto with coqlib.
+  destruct (zeq max min); simpl.
+  replace n with k1 by lia. rewrite zeq_true; auto.
+  destruct (zeq n k1); auto.
+Qed.
+
+Lemma compile_tree_2_correct:
+  forall dfl k1 a1 k2 a2 min max n,
+  sorted ((k1, a1) :: (k2, a2) :: nil) ->
+  (forall k a, In (k, a) ((k1, a1) :: (k2, a2) :: nil) -> min <= k <= max) ->
+  min <= n <= max ->
+  comptree_match n (compile_tree_2 dfl k1 a1 k2 a2 min max) =
+  Some (switch_target n dfl ((k1, a1) :: (k2, a2) :: nil)).
+Proof.
+  intros. inv H.
+  assert (min <= k1 <= max) by eauto with coqlib.
+  assert (min <= k2 <= max) by eauto with coqlib.
+  assert (k1 < k2) by eauto with coqlib.
+  unfold compile_tree_2; simpl.
+  destruct (zeq n k1). auto.
+  destruct (zeq (max - min) 1).
+  replace n with k2 by lia. rewrite zeq_true; auto.
+  simpl. destruct (zeq n k2); auto.
+Qed.
+
+Lemma compile_tree_3_correct:
+  forall dfl k1 a1 k2 a2 k3 a3 min max n,
+  sorted ((k1, a1) :: (k2, a2) :: (k3, a3) :: nil) ->
+  (forall k a, In (k, a) ((k1, a1) :: (k2, a2) :: (k3, a3) :: nil) -> min <= k <= max) ->
+  min <= n <= max ->
+  comptree_match n (compile_tree_3 dfl k1 a1 k2 a2 k3 a3 min max) =
+  Some (switch_target n dfl ((k1, a1) :: (k2, a2) :: (k3, a3) :: nil)).
+Proof.
+  intros. inv H. inv H4.
+  assert (min <= k1 <= max) by eauto with coqlib.
+  assert (min <= k2 <= max) by eauto with coqlib.
+  assert (min <= k3 <= max) by eauto with coqlib.
+  assert (k1 < k2) by eauto with coqlib.
+  assert (k2 < k3) by eauto with coqlib.
+  unfold compile_tree_3; simpl.
+  destruct (zeq n k1). auto.
+  destruct (zeq n k2). auto.
+  destruct (zeq (max - min) 2).
+  replace n with k3 by lia. rewrite zeq_true; auto.
+  simpl. destruct (zeq n k3); auto.
+Qed.
+
+Lemma compile_tree_correct:
+  forall n dfl tbl min max,
+  sorted tbl ->
+  (forall k a, In (k, a) tbl -> min <= k <= max) ->
+  min <= n <= max ->
+  comptree_match n (compile_tree dfl tbl min max) = Some(switch_target n dfl tbl).
+Proof.
+  intros until max. functional induction (compile_tree dfl tbl min max); intros SS R1 R2.
+- (* empty *)
+  simpl. auto.
+- (* one case *)
+  apply compile_tree_1_correct; auto.
+- (* two cases *)
+  apply compile_tree_2_correct; auto.
+- (* three cases *)
+  apply compile_tree_3_correct; auto.
+- (* N cases *)
+  set (pivot := first_key tbl2) in *.
+  assert (TBL2: tbl2 <> nil).
+  { destruct tbl as [ | [k1 a1] tbl]; try contradiction.
+    destruct tbl as [ | [k2 a2] tbl]; try contradiction.
+    destruct (split_in_half_length' (k1,a1) (k2,a2) tbl) as [P Q].
+    rewrite e0 in Q. destruct tbl2; simpl in Q. lia. congruence. }
+  assert (A: exists apivot tbl3, tbl2 = (pivot, apivot) :: tbl3).
+  { destruct tbl2 as [ | [k a] tbl3]. congruence. unfold pivot; simpl. exists a, tbl3; auto. }
+  destruct A as (apivot & tbl3 & EQ2).   
+  clear y.
+  generalize (split_in_half_eq tbl). rewrite e0; simpl. intros EQ.
+  destruct (sorted_app_inv tbl1 tbl2) as (SS1 & SS2 & SEP).
+  rewrite EQ; auto.
+  assert (R11: forall k a, In (k, a) tbl1 -> min <= k <= pivot - 1).
+  { intros. 
+    assert (min <= k <= max).
+    { apply R1 with a. rewrite <- EQ. apply in_or_app; auto. }
+    assert (k < pivot).
+    { eapply SEP. eauto. rewrite EQ2; eauto with coqlib. }
+    lia. }
+  assert (R12: forall k a, In (k, a) tbl2 -> pivot <= k <= max).
+  { intros. 
+    assert (min <= k <= max).
+    { apply R1 with a. rewrite <- EQ. apply in_or_app; auto. }
+    assert (pivot <= k).
+    { eapply in_sorted_le. rewrite EQ2 in SS2. eexact SS2. rewrite <- EQ2. eexact H. }
+    lia. }
+  simpl. destruct (zlt n pivot).
+  + assert (min <= n <= pivot - 1) by lia. rewrite IHc by eauto.
+    f_equal. symmetry; rewrite <- EQ. apply switch_target_app_1. 
+    intros. apply R12 in H0. lia.
+  + assert (pivot <= n <= max) by lia. rewrite IHc0 by eauto.
+    f_equal. symmetry; rewrite <- EQ. apply switch_target_app_2.
+    intros. apply R11 in H0. lia.
+Qed.
+
+Lemma compile_tree_wf:
+  forall dfl tbl min max,
+  (forall k a, In (k, a) tbl -> 0 <= k < modulus) ->
+  wf_comptree (compile_tree dfl tbl min max).
+Proof.
+  intros until max.  functional induction (compile_tree dfl tbl min max); intros R.
 - constructor.
-- destruct (split_eq key cases) as [[act'|] others]; try discriminate; InvBooleans.
-  constructor; eauto.
-- destruct (split_lt key cases) as [lc rc]; InvBooleans.
-  constructor; eauto.
-- destruct (split_between default ofs sz cases) as [ins out]; InvBooleans.
-  constructor; eauto.
+- unfold compile_tree_1. destruct (zeq max min); eauto using wf_comptree with coqlib.
+- unfold compile_tree_2. constructor. eauto with coqlib.
+  destruct (zeq (max - min) 1); eauto using wf_comptree with coqlib.
+- unfold compile_tree_3. constructor. eauto with coqlib.
+  constructor. eauto with coqlib.
+  destruct (zeq (max - min) 2); eauto using wf_comptree with coqlib.
+- clear y. generalize (split_in_half_eq tbl). rewrite e0; simpl. intros EQ.
+  constructor.
+  destruct tbl2 as [ | [key2 act2] tbl2 ]; simpl. lia.
+  apply R with act2. rewrite <- EQ; apply in_or_app; auto with coqlib.
+  apply IHc. intros; eapply R; rewrite <- EQ; apply in_or_app; eauto.
+  apply IHc0. intros; eapply R; rewrite <- EQ; apply in_or_app; eauto.
 Qed.
 
-(** Semantic correctness proof for validation. *)
+(** Final results *)
 
-Lemma split_eq_prop:
-  forall v default n cases optact cases',
-  split_eq n cases = (optact, cases') ->
-  switch_target v default cases =
-   (if zeq v n
-    then match optact with Some act => act | None => default end
-    else switch_target v default cases').
+Theorem compile_switch_correct:
+  forall dfl tbl n,
+  0 <= n < modulus ->
+  comptree_match n (compile_switch modulus dfl tbl) = Some(switch_target n dfl tbl).
 Proof.
-  induction cases; simpl; intros until cases'.
-- intros. inv H. simpl. destruct (zeq v n); auto.
-- destruct a as [key act].
-  destruct (split_eq n cases) as [same other] eqn:SEQ.
-  rewrite (IHcases same other) by auto.
-  destruct (zeq key n); intros EQ; inv EQ.
-+ destruct (zeq v n); auto.
-+ simpl. destruct (zeq v key).
-  * subst v. rewrite zeq_false by auto. auto.
-  * auto.
+  intros until n. intros RANGE. unfold compile_switch.
+  set (tbl1 := normalize_table modulus tbl).
+  assert (SRT: sorted tbl1) by (apply normalize_table_sorted).
+  assert (R1: forall k a, In (k, a) tbl1 -> 0 <= k < modulus) by (apply normalize_table_wf).
+  rewrite <- normalize_table_correct by auto. fold tbl1.
+  destruct tbl1 as [ | [kmin amin] l ].
+- (* empty table *)
+  reflexivity.
+- (* nonempty table *)
+  clear tbl. set (tbl := (kmin, amin) :: l) in *.
+  assert (E: tbl = removelast tbl ++ last tbl (kmin, amin) :: nil).
+  { apply app_removelast_last. unfold tbl; congruence. }
+  destruct (last tbl (kmin, amin)) as [kmax amax].
+  assert (R2: forall k a, In (k, a) tbl -> kmin <= k <= kmax).
+  { intros; split. 
+    eapply in_sorted_le; eassumption.
+    eapply in_sorted_ge. rewrite E in SRT; eauto. rewrite E in H; eauto. }
+  destruct (dense_enough (list_length_z tbl) (kmax - kmin + 1)) eqn:D.
++ apply compile_jumptable_correct; auto. 
+  eapply R1. unfold tbl; eauto with coqlib. 
+  eapply R2. unfold tbl; eauto with coqlib. 
+  eapply R1. rewrite E. apply in_or_app. eauto with coqlib.
+  unfold dense_enough in D. InvBooleans. auto. 
++ apply compile_tree_correct; auto.
+  intros. exploit R1; eauto. lia. 
+  lia.
 Qed.
 
-Lemma split_lt_prop:
-  forall v default n cases lcases rcases,
-  split_lt n cases = (lcases, rcases) ->
-  switch_target v default cases =
-    (if zlt v n
-     then switch_target v default lcases
-     else switch_target v default rcases).
+Theorem compile_switch_wf:
+  forall dfl tbl, 
+  Int.modulus <= modulus ->
+  wf_comptree (compile_switch modulus dfl tbl).
 Proof.
-  induction cases; intros until rcases; simpl.
-- intros. inv H. simpl. destruct (zlt v n); auto.
-- destruct a as [key act].
-  destruct (split_lt n cases) as [lc rc] eqn:SEQ.
-  rewrite (IHcases lc rc) by auto.
-  destruct (zlt key n); intros EQ; inv EQ; simpl.
-+ destruct (zeq v key). rewrite zlt_true by lia. auto. auto.
-+ destruct (zeq v key). rewrite zlt_false by lia. auto. auto.
-Qed.
-
-Lemma split_between_prop:
-  forall v default ofs sz cases inside outside,
-  split_between default ofs sz cases = (inside, outside) ->
-  switch_target v default cases =
-    (if zlt ((v - ofs) mod modulus) sz
-     then ZMap.get v inside
-     else switch_target v default outside).
-Proof.
-  induction cases; intros until outside; simpl; intros SEQ.
-- inv SEQ. rewrite ZMap.gi. simpl. destruct (zlt ((v - ofs) mod modulus) sz); auto.
-- destruct a as [key act].
-  destruct (split_between default ofs sz cases) as [ins outs].
-  erewrite IHcases; eauto.
-  destruct (zlt ((key - ofs) mod modulus) sz); inv SEQ.
-+ rewrite ZMap.gsspec. unfold ZIndexed.eq.
-  destruct (zeq v key).
-  subst v. rewrite zlt_true by auto. auto.
-  auto.
-+ simpl. destruct (zeq v key).
-  subst v. rewrite zlt_false by auto. auto.
-  auto.
-Qed.
-
-Lemma validate_jumptable_correct_rec:
-  forall cases tbl base v,
-  validate_jumptable cases tbl base = true ->
-  0 <= v < list_length_z tbl ->
-  list_nth_z tbl v = Some(ZMap.get (base + v) cases).
-Proof.
-  induction tbl; simpl; intros.
-- unfold list_length_z in H0. simpl in H0. extlia.
-- InvBooleans. rewrite list_length_z_cons in H0. apply Nat.eqb_eq in H1.
-  destruct (zeq v 0).
-  + replace (base + v) with base by lia. congruence.
-  + replace (base + v) with (Z.succ base + Z.pred v) by lia.
-    apply IHtbl. auto. lia.
-Qed.
-
-Lemma validate_jumptable_correct:
-  forall cases tbl ofs v sz,
-  validate_jumptable cases tbl ofs = true ->
-  (v - ofs) mod modulus < sz ->
-  0 <= sz -> 0 <= ofs -> ofs + sz <= modulus ->
-  0 <= v < modulus ->
-  sz <= list_length_z tbl ->
-  list_nth_z tbl ((v - ofs) mod modulus) = Some(ZMap.get v cases).
-Proof.
-  intros.
-  rewrite (validate_jumptable_correct_rec cases tbl ofs); auto.
-- f_equal. f_equal. rewrite Z.mod_small. lia.
-  destruct (zle ofs v). lia.
-  assert (M: ((v - ofs) + 1 * modulus) mod modulus = (v - ofs) + modulus).
-  { rewrite Z.mod_small. lia. lia. }
-  rewrite Z_mod_plus in M by auto. rewrite M in H0. lia.
-- generalize (Z_mod_lt (v - ofs) modulus modulus_pos). lia.
-Qed.
-
-Lemma validate_correct_rec:
-  forall default v,
-  0 <= v < modulus ->
-  forall t cases lo hi,
-  validate default cases t lo hi = true ->
-  lo <= v <= hi ->
-  comptree_match v t = Some (switch_target v default cases).
-Proof.
-  intros default v VRANGE. induction t; simpl; intros until hi.
-- (* base case *)
-  destruct cases as [ | [key1 act1] cases1]; intros.
-+ apply Nat.eqb_eq in H. subst act. reflexivity.
-+ InvBooleans. apply Nat.eqb_eq in H2. subst. simpl.
-  destruct (zeq v hi). auto. extlia.
-- (* eq node *)
-  destruct (split_eq key cases) as [optact others] eqn:EQ. intros.
-  destruct optact as [act1|]; InvBooleans; try discriminate.
-  apply Nat.eqb_eq in H.
-  rewrite (split_eq_prop v default _ _ _ _ EQ).
-  destruct (zeq v key).
-  + congruence.
-  + eapply IHt; eauto.
-    unfold refine_low_bound, refine_high_bound. split.
-    destruct (zeq key lo); lia.
-    destruct (zeq key hi); lia.
-- (* lt node *)
-  destruct (split_lt key cases) as [lcases rcases] eqn:EQ; intros; InvBooleans.
-  rewrite (split_lt_prop v default _ _ _ _ EQ). destruct (zlt v key).
-  eapply IHt1. eauto. lia.
-  eapply IHt2. eauto. lia.
-- (* jumptable node *)
-  destruct (split_between default ofs sz cases) as [ins outs] eqn:EQ; intros; InvBooleans.
-  rewrite (split_between_prop v _ _ _ _ _ _ EQ).
-  assert (0 <= (v - ofs) mod modulus < modulus) by (apply Z_mod_lt; lia).
-  destruct (zlt ((v - ofs) mod modulus) sz).
-  rewrite Z.mod_small by lia. eapply validate_jumptable_correct; eauto.
-  eapply IHt; eauto.
-Qed.
-
-Definition table_tree_agree
-    (default: nat) (cases: table) (t: comptree) : Prop :=
-  forall v, 0 <= v < modulus -> comptree_match v t = Some(switch_target v default cases).
-
-Theorem validate_switch_correct:
-  forall default t cases,
-  validate_switch default cases t = true ->
-  wf_comptree t /\ table_tree_agree default cases t.
-Proof.
-  unfold validate_switch, table_tree_agree; split.
-  eapply validate_wf; eauto.
-  intros; eapply validate_correct_rec; eauto. lia.
+  intros until tbl; intros MOD. unfold compile_switch.
+  set (tbl1 := normalize_table modulus tbl).
+  assert (SRT: sorted tbl1) by (apply normalize_table_sorted).
+  assert (R1: forall k a, In (k, a) tbl1 -> 0 <= k < modulus) by (apply normalize_table_wf).
+  destruct tbl1 as [ | [kmin amin] l ].
+- (* empty table *)
+  constructor.
+- (* nonempty table *)
+  clear tbl. set (tbl := (kmin, amin) :: l) in *.
+  assert (E: tbl = removelast tbl ++ last tbl (kmin, amin) :: nil).
+  { apply app_removelast_last. unfold tbl; congruence. }
+  destruct (last tbl (kmin, amin)) as [kmax amax].
+  assert (R2: forall k a, In (k, a) tbl -> kmin <= k <= kmax).
+  { intros; split.
+    eapply in_sorted_le; eassumption.
+    eapply in_sorted_ge. rewrite E in SRT; eauto. rewrite E in H; eauto. }
+  destruct (dense_enough (list_length_z tbl) (kmax - kmin + 1)) eqn:D.
++ apply compile_jumptable_wf; auto.
+  eapply R1. unfold tbl; eauto with coqlib. 
+  eapply R2. unfold tbl; eauto with coqlib. 
+  eapply R1. rewrite E. apply in_or_app. eauto with coqlib.
+  unfold dense_enough in D. InvBooleans. auto. 
++ apply compile_tree_wf; auto.
 Qed.
 
 End COMPTREE.
